Breaking up one big file

BasicSerializers.v
@@ -5,85 +5,242 @@ From StructTact Require Import StructTactics Fin.
 Require Fin Ascii.
 
 Require Import Cheerios.Core.
-Require Import Cheerios.Tactics.
 Require Import Cheerios.DeserializerMonad.
+Require Import Cheerios.Tactics.
 Import DeserializerNotations.
 
-Definition bool_serialize (b : bool) : list bool := [b].
+Lemma byte_serialize_deserialize_id :
+  serialize_deserialize_id_spec Serializer.putByte Deserializer.getByte.
+Proof. cheerios_crush. Qed.
 
-Definition bool_deserialize : deserializer bool :=
-  l <- get ;;
-  match l with
-  | [] => fail
-  | b :: l' => put l' ;; ret b
-  end.
+Instance byte_Serializer : Serializer byte :=
+  {| serialize := Serializer.putByte;
+     deserialize := Deserializer.getByte;
+     serialize_deserialize_id := byte_serialize_deserialize_id |}.
+
+Definition bool_serialize (b : bool) : Serializer.t :=
+  if b then serialize x01 else serialize x00.
+
+Definition bool_deserialize :=
+  b <- deserialize ;;
+    match b with
+    | x00 => Deserializer.ret false
+    | x01 => Deserializer.ret true
+    | _ => Deserializer.error
+    end.
 
 Lemma bool_serialize_deserialize_id :
   serialize_deserialize_id_spec bool_serialize bool_deserialize.
 Proof.
-  destruct a; auto.
+  intros.
+  unfold bool_serialize, bool_deserialize.
+  destruct a;
+    cheerios_crush; simpl; cheerios_crush.
 Qed.
 
 Instance bool_Serializer : Serializer bool :=
   {| serialize := bool_serialize;
      deserialize := bool_deserialize;
-     serialize_deserialize_id := bool_serialize_deserialize_id
-  |}.
+     serialize_deserialize_id := bool_serialize_deserialize_id |}.
 
-
-(* This is about 2x less space-efficient than necessary, since it outputs two
-   bits for every "bit" in the input, but it's very easy to verify. *)
-Fixpoint positive_serialize (p : positive) : list bool :=
-  match p with
-  | xI p' => serialize true ++ serialize true ++ positive_serialize p'
-  | xO p' => serialize true ++ serialize false ++ positive_serialize p'
-  | xH => serialize false
-  end.
-
-(* This has to be implemented directly on the implementation of Deserializer.t
-   because it performs recursion on the underlying list of bits. *)
-Fixpoint positive_deserialize (l : list bool) : option (positive * list bool) :=
-  match l with
-  | [] => None
-  | continue :: l' =>
-    if continue
-    then match l' with
-         | [] => None
-         | bit :: l' => match positive_deserialize l' with None => None
-                       | Some (p, l') => Some ((if bit then xI else xO) p, l')
-                       end
-         end
-    else Some (xH, l')
-  end.
-
-Lemma positive_serialize_deserialize_id :
-  forall p bin, positive_deserialize (positive_serialize p ++ bin) = Some (p, bin).
+(* this needs to go here because we need the bool_Serializer instance *)
+Lemma fold_append_unwrap :
+  forall {S A : Type}
+         (f : byte -> S -> fold_state S A) (s : S)
+         (b : byte) (tail : Serializer.t) (bin : list byte),
+    Deserializer.unwrap (Deserializer.fold f s)
+                        (Serializer.unwrap (Serializer.append
+                                              (serialize b)
+                                              tail) ++ bin) =
+    match f b s with
+    | Done a => Some(a, Serializer.unwrap tail ++ bin)
+    | More s => Deserializer.unwrap (Deserializer.fold f s)
+                                    (Serializer.unwrap tail ++ bin)
+    | Error => None
+    end.
 Proof.
-  induction p; simpl; intros; auto; rewrite IHp; auto.
+  cheerios_crush.
 Qed.
 
-Instance positive_Serializer : Serializer positive :=
-  {| serialize := positive_serialize;
-     deserialize := positive_deserialize;
-     serialize_deserialize_id := positive_serialize_deserialize_id
-  |}.
+Lemma fold_append_unwrap' :
+  forall {S A : Type}
+         (f : byte -> S -> fold_state S A) (s : S)
+         (b : byte) (tail : Serializer.t) (bin : list byte),
+    Deserializer.unwrap (Deserializer.fold f s)
+                        (Serializer.unwrap (Serializer.append
+                                              (Serializer.putByte b)
+                                              tail) ++ bin) =
+  match f b s with
+    | Done a => Some(a, Serializer.unwrap tail ++ bin)
+    | More s => Deserializer.unwrap (Deserializer.fold f s)
+                                    (Serializer.unwrap tail ++ bin)
+    | Error => None
+    end.
+Proof.
+  cheerios_crush.
+Qed.
+Hint Rewrite @fold_append_unwrap @fold_append_unwrap' : cheerios.
 
-(* This is the first example of a "typical" serializer: it combines more
-   primitive serializers (in this case, just for bool and positive) together in
-   order to serialize a Z. *)
-Definition Z_serialize (z : Z) : list bool :=
-  match z with
-  | Z0 => serialize false
-  | Zpos p => serialize true ++ serialize true ++ serialize p
-  | Zneg p => serialize true ++ serialize false ++ serialize p
+
+Inductive le_pos (p : positive) : positive -> Prop :=
+| le_p : le_pos p p
+| le_xI : forall p2, le_pos p p2 -> le_pos p (xI p2)
+| le_xO : forall p2, le_pos p p2 -> le_pos p (xO p2).
+
+Section PositiveInductionPrinciple.
+  Variable P : positive -> Prop.
+
+  Lemma strongind_pos_aux :
+    P xH ->
+    (forall q, ((forall p, le_pos p q -> P p) -> P (xI q)) /\
+               ((forall p, le_pos p q -> P p) -> P (xO q))) ->
+    (forall q, (forall p, le_pos p q -> P p)).
+  Proof.
+    induction q;
+      intros;
+      inversion H1;
+      auto;
+      apply H0;
+      apply IHq.
+  Qed.
+
+  Lemma weaken_pos :
+    (forall q, (forall p, le_pos p q -> P p)) -> forall p, P p.
+  Proof.
+    intros.
+    apply (H p p).
+    constructor.
+  Qed.
+
+  Theorem strongind_pos :
+    P xH ->
+    (forall q, ((forall p, le_pos p q -> P p) -> P (xI q)) /\
+               ((forall p, le_pos p q -> P p) -> P (xO q))) ->
+    forall p, P p.
+  Proof.
+    intros.
+    apply weaken_pos.
+    now apply strongind_pos_aux.
+  Qed.
+End PositiveInductionPrinciple.
+
+Local Open Scope char_scope.
+
+Fixpoint positive_serialize p :=
+  match p with
+  | xI (xI (xI p)) => Serializer.append (serialize x0e)
+                                        (positive_serialize p)
+  | xI (xI (xO p)) => Serializer.append (serialize x0d)
+                                        (positive_serialize p)
+  | xI (xO (xI p)) => Serializer.append (serialize x0c)
+                                        (positive_serialize p)
+  | xI (xO (xO p)) => Serializer.append (serialize x0b)
+                                        (positive_serialize p)
+  | xO (xI (xI p)) => Serializer.append (serialize x0a)
+                                        (positive_serialize p)
+  | xO (xI (xO p)) => Serializer.append (serialize x09)
+                                        (positive_serialize p)
+  | xO (xO (xI p)) => Serializer.append (serialize x08)
+                                        (positive_serialize p)
+  | xO (xO (xO p)) => Serializer.append (serialize x07)
+                                        (positive_serialize p)
+  | xI (xI p) => Serializer.append (serialize x06)
+                                   (positive_serialize p)
+  | xI (xO p) => Serializer.append (serialize x05)
+                                   (positive_serialize p)
+  | xO (xI p) => Serializer.append (serialize x04)
+                                   (positive_serialize p)
+  | xO (xO p) => Serializer.append (serialize x03)
+                                   (positive_serialize p)
+  | xI p => Serializer.append (serialize x02)
+                              (positive_serialize p)
+  | xO p => Serializer.append (serialize x01)
+                              (positive_serialize p)
+  | XH => serialize x00
   end.
 
-Definition Z_deserialize : deserializer Z :=
+Definition depositive_serialize_step
+           (b : byte)
+           (s : positive -> positive) := 
+  match b with
+  | x0e => More (fun p => s (xI (xI (xI p))))
+  | x0d => More (fun p => s (xI (xI (xO p))))
+  | x0c => More (fun p => s (xI (xO (xI p))))
+  | x0b => More (fun p => s (xI (xO (xO p))))
+  | x0a => More (fun p => s (xO (xI (xI p))))
+  | x09 => More (fun p => s (xO (xI (xO p))))
+  | x08 => More (fun p =>  s (xO (xO (xI p))))
+  | x07 => More (fun p => s (xO (xO (xO p))))
+  | x06 => More (fun p => s (xI (xI p)))
+  | x05 => More (fun p => s (xI (xO p)))
+  | x04 => More (fun p => s (xO (xI p)))
+  | x03 => More (fun p => s (xO (xO p)))
+  | x02 => More (fun p => s (xI p))
+  | x01 => More (fun p => s (xO p))
+  | x00 => Done (s xH)
+  | _ => Error
+  end.
+
+Definition positive_step_aux p :=
+  forall (k : positive -> positive) (bytes : list byte),
+    Deserializer.unwrap (Deserializer.fold depositive_serialize_step k)
+                        (Serializer.unwrap (positive_serialize p) ++ bytes)
+    = Some(k p, bytes).
+
+Lemma positive_step :
+  forall (p : positive), positive_step_aux p.
+Proof.
+  apply strongind_pos; unfold positive_step_aux.
+  - unfold positive_serialize.
+    cheerios_crush.
+  - split;
+      intros;
+      try destruct q;
+      try destruct q;
+      simpl; cheerios_crush; simpl; rewrite H || cheerios_crush;
+        try reflexivity;
+        repeat constructor.
+Qed.
+
+Definition depositive_serialize :=
+  Deserializer.fold depositive_serialize_step (fun p => p).
+
+Theorem serialize_depositive_serialize_id :
+  serialize_deserialize_id_spec positive_serialize
+                                depositive_serialize.
+Proof.
+  intros.
+  unfold depositive_serialize.
+  apply positive_step.
+Qed.
+
+Instance positive_Serializer : Serializer positive.
+Proof.
+  exact ({| serialize := positive_serialize;
+            deserialize := depositive_serialize;
+            serialize_deserialize_id := serialize_depositive_serialize_id
+         |}).
+Qed.
+
+
+
+(* This is the first example of a "typical" serializer: it combines more
+   primitive serializers (in this case, just for byte and positive) together in
+   order to serialize a Z. *)
+Definition Z_serialize (z : Z) : Serializer.t :=
+  match z with
+  | Z0 => serialize x00
+  | Zpos p => Serializer.append (serialize x01) (serialize p)
+  | Zneg p => Serializer.append (serialize x02) (serialize p)
+  end.
+
+Definition Z_deserialize : Deserializer.t Z :=
   tag <- deserialize ;;
   match tag with
-  | true => sign <- deserialize ;;
-           (match sign with true => Zpos | false => Zneg end) <$> deserialize
-  | false => ret Z0
+  | x02 => Zneg <$> deserialize
+  | x01 => Zpos <$> deserialize
+  | x00 => Deserializer.ret Z0
+  | _ => Deserializer.error
   end.
 
 (* This proof is typical for serializing an algebraic datatype. Unfold the
@@ -92,8 +249,10 @@ Definition Z_deserialize : deserializer Z :=
 Lemma Z_serialize_deserialize_id :
   serialize_deserialize_id_spec Z_serialize Z_deserialize.
 Proof.
+  intros.
   unfold Z_serialize, Z_deserialize.
-  destruct a; serialize_deserialize_id_crush.
+  destruct a;
+   repeat (cheerios_crush; simpl).
 Qed.
 
 Instance Z_Serializer : Serializer Z :=
@@ -102,25 +261,26 @@ Instance Z_Serializer : Serializer Z :=
      serialize_deserialize_id := Z_serialize_deserialize_id
   |}.
 
-
-Definition N_serialize (n : N) : list bool :=
+Definition N_serialize n :=
   match n with
   | N0 => serialize false
-  | Npos p => serialize true ++ serialize p
+  | Npos p => Serializer.append (serialize true) (serialize p)
   end.
 
-Definition N_deserialize : deserializer N :=
+Definition N_deserialize : Deserializer.t N :=
   tag <- deserialize ;;
   match tag with
-  | false => ret N0
+  | false => Deserializer.ret N0
   | true => Npos <$> deserialize
   end.
 
 Lemma N_serialize_deserialize_id :
   serialize_deserialize_id_spec N_serialize N_deserialize.
 Proof.
+  intros.
   unfold N_serialize, N_deserialize.
-  destruct a; serialize_deserialize_id_crush.
+  destruct a;
+    repeat (cheerios_crush; simpl).
 Qed.
 
 Instance N_Serializer : Serializer N :=
@@ -130,11 +290,14 @@ Instance N_Serializer : Serializer N :=
   |}.
 
 
+
+
 (* The other main way to define a serializer is to use an isomorphism to another
    type that is already serializable. *)
-Definition nat_serialize (n : nat) : list bool := serialize (N.of_nat n).
+Definition nat_serialize n : Serializer.t := serialize (N.of_nat n).
 
-Definition nat_deserialize : deserializer nat := N.to_nat <$> deserialize.
+Definition nat_deserialize : Deserializer.t nat := N.to_nat <$> deserialize.
+
 
 (* This proof is typical for serializers defined by converting to and from a
    type that is already serializable. Unfold the serializer and deserializer,
@@ -144,7 +307,7 @@ Lemma nat_serialize_deserialize_id :
   serialize_deserialize_id_spec nat_serialize nat_deserialize.
 Proof.
   unfold nat_serialize, nat_deserialize.
-  serialize_deserialize_id_crush.
+  cheerios_crush.
   now rewrite Nnat.Nat2N.id.
 Qed.
 
@@ -154,16 +317,15 @@ Instance nat_Serializer : Serializer nat :=
      serialize_deserialize_id := nat_serialize_deserialize_id
   |}.
 
-
 (* Serializer for the standard library's Fin.t based on converting to nat. *)
-Definition Fin_serialize {n} (x : Fin.t n) : list bool :=
+Definition Fin_serialize {n} (x : Fin.t n) : Serializer.t :=
   serialize (proj1_sig (Fin.to_nat x)).
 
-Definition Fin_deserialize {n} : deserializer (Fin.t n) :=
+Definition Fin_deserialize {n} : Deserializer.t (Fin.t n) :=
   m <- deserialize ;;
     match Fin.of_nat m n with
-    | inleft x => ret x
-    | inright _ => fail
+    | inleft x => Deserializer.ret x
+    | inright _ => Deserializer.error
     end.
 
 Lemma Fin_of_nat_to_nat:
@@ -178,8 +340,9 @@ Qed.
 Lemma Fin_serialize_deserialize_id n : serialize_deserialize_id_spec Fin_serialize (@Fin_deserialize n).
 Proof.
   unfold Fin_serialize, Fin_deserialize.
-  serialize_deserialize_id_crush.
-  now rewrite Fin_of_nat_to_nat.
+  cheerios_crush.
+  rewrite Fin_of_nat_to_nat.
+  cheerios_crush.
 Qed.
 
 Instance Fin_Serializer n : Serializer (Fin.t n) :=
@@ -188,23 +351,23 @@ Instance Fin_Serializer n : Serializer (Fin.t n) :=
      serialize_deserialize_id := Fin_serialize_deserialize_id n
   |}.
 
-
 (* Serializer for StructTact's fin based on converting to nat. *)
-Definition fin_serialize {n} (x : fin n) : list bool :=
+Definition fin_serialize {n} (x : fin n) : Serializer.t :=
   serialize (fin_to_nat x).
 
-Definition fin_deserialize {n} : deserializer (fin n) :=
+Definition fin_deserialize {n} : Deserializer.t (fin n) :=
   m <- deserialize ;;
     match fin_of_nat m n with
-    | inleft x => ret x
-    | inright _ => fail
+    | inleft x => Deserializer.ret x
+    | inright _ => Deserializer.error
     end.
 
 Lemma fin_serialize_deserialize_id n : serialize_deserialize_id_spec fin_serialize (@fin_deserialize n).
 Proof.
   unfold fin_serialize, fin_deserialize.
-  serialize_deserialize_id_crush.
-  now rewrite fin_of_nat_fin_to_nat.
+  cheerios_crush.
+  rewrite fin_of_nat_fin_to_nat.
+  cheerios_crush.
 Qed.
 
 Instance fin_Serializer n : Serializer (fin n) :=
@@ -213,18 +376,17 @@ Instance fin_Serializer n : Serializer (fin n) :=
      serialize_deserialize_id := fin_serialize_deserialize_id n
   |}.
 
-
-Definition ascii_serialize (a : Ascii.ascii) : list bool :=
+Definition ascii_serialize (a : Ascii.ascii) : Serializer.t :=
   serialize (Ascii.nat_of_ascii a).
 
-Definition ascii_deserialize : deserializer Ascii.ascii :=
+Definition ascii_deserialize : Deserializer.t Ascii.ascii :=
   Ascii.ascii_of_nat <$> deserialize.
 
 Lemma ascii_serialize_deserialize_id :
   serialize_deserialize_id_spec ascii_serialize ascii_deserialize.
 Proof.
   unfold ascii_deserialize, ascii_serialize.
-  serialize_deserialize_id_crush.
+  cheerios_crush.
   now rewrite Ascii.ascii_nat_embedding.
 Qed.
 
