Core.v
@@ -1,8 +1,209 @@
 Require Import List.
 Import ListNotations.
 
+Require Import Ascii List ZArith.
+Import ListNotations.
+Set Implicit Arguments.
+
+Inductive fold_state S A :=
+| Done (a : A)
+| More (s : S)
+| Error.
+Arguments Done {_} {_} _.
+Arguments More {_} {_} _.
+Arguments Error {_} {_}.
+
+Inductive byte :=
+| x00 | x01 | x02 | x03 | x04 | x05 | x06 | x07 | x08 | x09 | x0a | x0b | x0c
+| x0d | x0e | x0f | x10 | x11 | x12 | x13 | x14 | x15 | x16 | x17 | x18 | x19
+| x1a | x1b | x1c | x1d | x1e | x1f | x20 | x21 | x22 | x23 | x24 | x25 | x26
+| x27 | x28 | x29 | x2a | x2b | x2c | x2d | x2e | x2f | x30 | x31 | x32 | x33
+| x34 | x35 | x36 | x37 | x38 | x39 | x3a | x3b | x3c | x3d | x3e | x3f | x40
+| x41 | x42 | x43 | x44 | x45 | x46 | x47 | x48 | x49 | x4a | x4b | x4c | x4d
+| x4e | x4f | x50 | x51 | x52 | x53 | x54 | x55 | x56 | x57 | x58 | x59 | x5a
+| x5b | x5c | x5d | x5e | x5f | x60 | x61 | x62 | x63 | x64 | x65 | x66 | x67
+| x68 | x69 | x6a | x6b | x6c | x6d | x6e | x6f | x70 | x71 | x72 | x73 | x74
+| x75 | x76 | x77 | x78 | x79 | x7a | x7b | x7c | x7d | x7e | x7f | x80 | x81
+| x82 | x83 | x84 | x85 | x86 | x87 | x88 | x89 | x8a | x8b | x8c | x8d | x8e
+| x8f | x90 | x91 | x92 | x93 | x94 | x95 | x96 | x97 | x98 | x99 | x9a | x9b
+| x9c | x9d | x9e | x9f | xa0 | xa1 | xa2 | xa3 | xa4 | xa5 | xa6 | xa7 | xa8
+| xa9 | xaa | xab | xac | xad | xae | xaf | xb0 | xb1 | xb2 | xb3 | xb4 | xb5
+| xb6 | xb7 | xb8 | xb9 | xba | xbb | xbc | xbd | xbe | xbf | xc0 | xc1 | xc2
+| xc3 | xc4 | xc5 | xc6 | xc7 | xc8 | xc9 | xca | xcb | xcc | xcd | xce | xcf
+| xd0 | xd1 | xd2 | xd3 | xd4 | xd5 | xd6 | xd7 | xd8 | xd9 | xda | xdb | xdc
+| xdd | xde | xdf | xe0 | xe1 | xe2 | xe3 | xe4 | xe5 | xe6 | xe7 | xe8 | xe9
+| xea | xeb | xec | xed | xee | xef | xf0 | xf1 | xf2 | xf3 | xf4 | xf5 | xf6
+| xf7 | xf8 | xf9 | xfa | xfb | xfc | xfd | xfe | xff.
+Module Type SERIALIZER.
+  Parameter t : Type.
+  Parameter empty : t.
+  Parameter append : t -> t -> t.
+  Parameter putByte : byte -> t.
+
+  (* For proof only! Do not call from serializers. *)
+  Parameter unwrap : t -> list byte.
+  Parameter empty_unwrap : unwrap empty = [].
+  Parameter append_unwrap :
+      forall x y : t, unwrap (append x y) = unwrap x ++ unwrap y.
+  Parameter putByte_unwrap : forall (a : byte), unwrap (putByte a) = [a].
+End SERIALIZER.
+
+Module Type DESERIALIZER.
+  Parameter t : Type -> Type.
+
+  Parameter getByte : t byte.
+  Parameter unwrap : forall A, t A -> list byte -> option (A * list byte).
+
+  Parameter getByte_unwrap : forall l,
+      unwrap getByte l = match l with
+                         | [] => None
+                         | a :: l => Some (a, l)
+                         end.
+
+  Parameter bind : forall A B, t A -> (A -> t B) -> t B.
+  Parameter ret : forall A, A -> t A.
+  Parameter map : forall A B, (A -> B) -> t A -> t B.
+  Parameter error : forall A, t A.
+
+  Parameter fold : forall S A,
+      (byte -> S -> fold_state S A) -> S -> t A.
+
+  Parameter bind_unwrap : forall A B (m : t A)
+                             (f : A -> t B) bytes,
+      unwrap (bind m f) bytes = match unwrap m bytes with
+                                | None => None
+                                | Some (v, bytes) => unwrap (f v) bytes
+                              end.
+  Parameter ret_unwrap : forall A (x: A) bytes, unwrap (ret x) bytes = Some (x, bytes).
+
+  Parameter map_unwrap: forall A B (f: A -> B) (d: t A) bin,
+      unwrap (map f d) bin =
+      match (unwrap d bin) with
+      | None => None
+      | Some (v, bin) => Some (f v, bin)
+      end.
+
+  Parameter fold_unwrap : forall {S A : Type}
+                             (f : byte -> S -> fold_state S A) (s : S) l,
+      unwrap (fold f s) l =
+      match l with
+      | [] => None
+      | b :: l => match f b s with
+                  | Done a => Some (a, l)
+                  | More s => unwrap (fold f s) l
+                  | Error => None
+                  end
+      end.
+End DESERIALIZER.
+
+  Module Serializer : SERIALIZER.
+    Definition t := list byte.
+  Definition empty : t := [].
+  Definition putByte (a : byte) : t := [a].
+
+  Definition append (x y : t) : t := x ++ y.
+
+  Definition unwrap (x : t) : list byte := x.
+
+  Lemma empty_unwrap : unwrap empty = [].
+  Proof. reflexivity. Qed.
+
+  Lemma putByte_unwrap : forall (a : byte), unwrap (putByte a) = [a].
+  Proof. reflexivity. Qed.
+
+  Lemma append_unwrap :
+    forall x y : t, unwrap (append x y) = unwrap x ++ unwrap y.
+  Proof. reflexivity. Qed.
+End Serializer.
+
+(* This is the monad used to write deserializers. It is a state monad with
+    failure, where the state is the serialized bits. *)
+
+Module Deserializer : DESERIALIZER.
+  Definition t (A : Type) := list byte -> option (A * list byte).
+  Definition unwrap {A} (x : t A) := x.
+
+  Definition getByte (l : list byte) :=
+    match l with
+    | [] => None
+    | b :: l => Some (b, l)
+    end.
+
+  Definition ret {A} (a : A) : t A := fun s => Some (a, s).
+
+  Definition bind {A B} (m : t A) (f : A -> t B) : t B :=
+    fun s => match m s with None => None
+                       | Some (a, s') => f a s'
+             end.
+
+  Definition map {A B} (f : A -> B) (d : Deserializer.t A) : Deserializer.t B :=
+    bind d (fun a => ret (f a)).
+
+  Definition error {A} : t A :=
+    fun l => None.
+
+  Lemma getByte_unwrap : forall l,
+      unwrap getByte l = match l with
+                         | [] => None
+                         | b :: l => Some (b, l)
+                        end.
+  Proof. reflexivity. Qed.
+
+  Lemma bind_unwrap : forall A B (m : t A)
+                             (f : A -> t B) bin,
+      unwrap (bind m f) bin = match unwrap m bin with
+                                | None => None
+                                | Some (v, bin) => unwrap (f v) bin
+                                end.
+  Proof.
+    unfold bind.
+    intros.
+    reflexivity.
+  Qed.
+
+  Fixpoint fold {S A}
+           (f : byte -> S -> fold_state S A) (s : S) (l : list byte) :=
+    match l with
+    | [] => None
+    | b :: l => match f b s with
+                | Done a => Some (a, l)
+                | More s => fold f s l
+                | Error => None
+                end
+    end.
+
+  Lemma ret_unwrap : forall {A} (x: A) bytes, unwrap (ret x) bytes = Some (x, bytes).
+  Proof. reflexivity. Qed.
+
+  Lemma map_unwrap: forall A B (f: A -> B) (d: Deserializer.t A) bin,
+      Deserializer.unwrap (map f d) bin =
+      match (Deserializer.unwrap d bin) with
+      | None => None
+      | Some (v, bin) => Some (f v, bin)
+      end.
+  Proof. reflexivity. Qed.
+
+  Lemma fold_unwrap : forall {S A : Type}
+                             (f : byte -> S -> fold_state S A) (s : S) l,
+      unwrap (fold f s) l =
+      match l with
+      | [] => None
+      | b :: l => match f b s with
+                  | Done a => Some (a, l)
+                  | More s => unwrap (fold f s) l
+                  | Error => None
+                  end
+      end.
+  Proof.
+    intros.
+    simpl. destruct l; reflexivity.
+  Qed.
+End Deserializer.
+Arguments Deserializer.error {_}.
+
 Notation serialize_deserialize_id_spec s d :=
-  (forall a (bin : list bool), d (s a ++ bin) = Some (a, bin)).
+  (forall a bin,
+      Deserializer.unwrap d (Serializer.unwrap (s a) ++ bin) = Some(a, bin)).
 
 (* This is the class of serializable types, which is the main entrypoint to
    Cheerios. Instances are required to show that `deserialize` can correctly
@@ -10,15 +211,17 @@ Notation serialize_deserialize_id_spec s d :=
    bitstream. *)
 Class Serializer (A : Type) : Type :=
   {
-    serialize : A -> list bool;
-    deserialize : list bool -> option (A * list bool);
+    serialize : A -> Serializer.t;
+    deserialize : Deserializer.t A;
     serialize_deserialize_id : serialize_deserialize_id_spec serialize deserialize
   }.
+Hint Rewrite @serialize_deserialize_id : cheerios.
 
 (* In particular, if there is nothing else in the bitsream, then deserialize and
    serialize are inverses. *)
 Lemma serialize_deserialize_id_nil :
-  forall A (sA : Serializer A) a, deserialize (serialize a) = Some (a, []).
+  forall A (sA : Serializer A) a,
+    Deserializer.unwrap deserialize (Serializer.unwrap (serialize a)) = Some (a, []).
 Proof.
   intros.
   pose proof serialize_deserialize_id a [].
