DeserializerMonad.v
@@ -1,45 +1,41 @@
 Require Import Cheerios.Core.
 Require Import List.
+Import ListNotations.
 
-(* This is the monad used to write deserializers. It is a state monad with
-    failure, where the state is the serialized bits. *)
-Definition deserializer (A : Type) : Type := list bool -> option (A * list bool).
+Definition sequence {A B} (df : Deserializer.t (A -> B))
+           (da : Deserializer.t A) : Deserializer.t B :=
+  Deserializer.bind df
+                    (fun f =>
+                          (Deserializer.bind da
+                                             (fun a => Deserializer.ret (f a)))).
 
-Definition ret {A} (a : A) : deserializer A := fun s => Some (a, s).
-
-Definition bind {A B} (m : deserializer A) (f : A -> deserializer B) : deserializer B :=
-  fun s => match m s with None => None
-                  | Some (a, s') => f a s'
-        end.
-
-Definition get : deserializer (list bool) := fun s => Some (s, s).
-
-Definition put (s : list bool) : deserializer unit := fun _ => Some (tt, s).
-
-Definition fail {A} : deserializer A := fun _ => None.
-
-(* useful for "undoing" a deserialize step *)
-Definition push (l : list bool) : deserializer unit := fun s => Some (tt, l ++ s).
-
-Definition fmap {A B} (f : A -> B) (x : deserializer A) : deserializer B :=
-  bind x (fun a => ret (f a)).
-
-Definition sequence {A B} (df : deserializer (A -> B)) (da : deserializer A) : deserializer B :=
-  bind df (fun f => (bind da (fun a => ret (f a)))).
+Lemma sequence_rewrite : forall {A B : Type}
+                                (df : Deserializer.t (A -> B))
+                                (da : Deserializer.t A),
+  sequence df da =
+  Deserializer.bind df
+                    (fun f =>
+                       (Deserializer.bind da
+                                          (fun a => Deserializer.ret (f a)))).
+Proof.
+  reflexivity.
+Qed.
+Hint Rewrite @sequence_rewrite : cheerios.
 
 Module DeserializerNotations.
-  Notation "m >>= f" := (@bind _ _ m f) (at level 42, left associativity).
+  Notation "m >>= f" := (@Deserializer.bind _ _ m f) (at level 42, left associativity).
 
   Notation "x <- c1 ;; c2" := (c1 >>= (fun x => c2))
                                 (at level 100, c1 at next level, right associativity).
   Notation "e1 ;; e2" := (_ <- e1 ;; e2)
                             (at level 100, right associativity).
 
-  Notation "f <$> x" := (@fmap _ _ f x) (at level 42, left associativity).
+  Notation "f <$> x" := (@Deserializer.map _ _ f x) (at level 42, left associativity).
 
   Notation "f <*> x" := (@sequence _ _ f x) (at level 42, left associativity).
 End DeserializerNotations.
 
+Check sequence.
 Import DeserializerNotations.
 
 Section lift.
@@ -48,16 +44,15 @@ Section lift.
   Context {sB : Serializer B}.
   Context {sC : Serializer C}.
   Context {sD : Serializer D}.
-
-  Definition liftD1 {X} (f : D -> X) : deserializer X :=
+  Definition liftD1 {X} (f : D -> X) :=
     f <$> deserialize.
 
-  Definition liftD2 {X} (f : C -> D -> X) : deserializer X :=
+  Definition liftD2 {X} (f : C -> D -> X) : Deserializer.t X :=
     (f <$> deserialize) >>= liftD1.
 
-  Definition liftD3 {X} (f : B -> C -> D -> X) : deserializer X :=
+  Definition liftD3 {X} (f : B -> C -> D -> X) : Deserializer.t X :=
     (f <$> deserialize) >>= liftD2.
 
-  Definition liftD4 {X} (f : A -> B -> C -> D -> X) : deserializer X :=
+  Definition liftD4 {X} (f : A -> B -> C -> D -> X) : Deserializer.t X :=
     (f <$> deserialize) >>= liftD3.
 End lift.
